client id type specified in Raft parameters

extraction/vard-log/ml/VarDLogSerialization.ml
@@ -7,10 +7,10 @@ open Util
 let outputToString out =
   match Obj.magic out with
   | NotLeader (client_id, request_id) ->
-    (client_id, sprintf "NotLeader %s" (string_of_int request_id))
+    (Obj.magic client_id, sprintf "NotLeader %s" (string_of_int request_id))
   | ClientResponse (client_id, request_id, o) ->
      let Response (k, value, old) = (Obj.magic o) in
-     (client_id,
+     (Obj.magic client_id,
       match (value, old) with
       | Some v, Some o ->
          sprintf "Response %s %s %s %s"
@@ -58,7 +58,7 @@ let deserializeInp buf =
 let deserializeInput inp client_id =
   match deserializeInp inp with
   | Some (request_id, input) ->
-    Some (ClientRequest (client_id, request_id, Obj.magic input))
+    Some (ClientRequest (Obj.magic client_id, request_id, Obj.magic input))
   | None -> None
 
 let deserializeClientId b =
