raft/RefinementSpecLemmas.v
@@ -215,7 +215,7 @@ Section SpecLemmas.
   Lemma update_elections_data_request_vote_reply_votesWithLog :
   forall  (h : name)
     (st : electionsData *
-          RaftState.raft_data term name entry logIndex serverType data output)
+          RaftState.raft_data term name entry logIndex serverType data clientId output)
     (src : name) (t : nat) (r : bool),
     votesWithLog (update_elections_data_requestVoteReply h src t r st) =
     votesWithLog (fst st).
@@ -576,7 +576,7 @@ Section SpecLemmas.
   Lemma update_elections_data_request_vote_votesWithLog_old :
     forall (h : name)
       (st : electionsData *
-            RaftState.raft_data term name entry logIndex serverType data output)
+            RaftState.raft_data term name entry logIndex serverType data clientId output)
       (t : nat) (src : fin N) (lli llt : nat)
       (t' : term) (h' : name) (l' : list entry),
       In (t', h', l') (votesWithLog (fst st)) ->
